Assignment 7. (a) (b)

Deduction.thy
@@ -2,6 +2,8 @@ theory Deduction imports
   Main Term
 begin
 
+(* 6. (a) *)
+
 definition intruder :: msg where
   "intruder = Cons ''intruder''"
 
@@ -22,28 +24,72 @@ lemma "{Sym_encrypt m x, x} \<turnstile> m"
 lemma "{Pair u1 u2} \<turnstile> Hash (Pair u1 u2)"
   by auto
 lemma "{Sym_encrypt m k, Public_key_encrypt k intruder} \<turnstile> Pair m (Signature m intruder)"
-  by (metis Adec Ax Pair Sdec Sig insertI1 insert_commute)
-(*  
-  apply(rule Pair)
-   apply(rule Sdec[of _ _ "k"], rule Ax, simp, rule Adec, rule Ax, simp)
-  by(rule Sig, rule Sdec[of _ _ "k"], rule Ax, simp, rule Adec, rule Ax, simp)
-*)
+  apply (rule Pair)
+   apply (rule Sdec)
+    prefer 2 apply (rule Adec)
+    prefer 3 apply (rule Sig)
+    apply (rule Sdec)
+     prefer 2 apply (rule Adec)
+  by auto
+
+(* 6. (b) *)
 
 lemma deduce_weaken:
   assumes "G \<turnstile> t" and "G \<subseteq> H"
   shows "H \<turnstile> t"
   using assms
-  by (induction rule: deduce.induct) auto+
+  by (induction rule: deduce.induct) auto
 
 lemma deduce_cut_aux:
   assumes "T \<turnstile> u" and "H \<turnstile> t" and "T = insert t H"
   shows "H \<turnstile> u"
   using assms
-  by(induction rule: deduce.induct) auto+
+  by (induction rule: deduce.induct) auto
 
 lemma deduce_cut:
   assumes "insert t H \<turnstile> u" and "H \<turnstile> t"
   shows "H \<turnstile> u"
   using assms deduce_cut_aux by blast
+
+(* 7. (a) *)
+
+datatype constraint = Constraint "msg list" "msg list" "msg" ("((2_/|_)/\<triangleright>_)" [67,67,67]66)
+type_synonym constraint_sys = "constraint set"
+
+fun c_fv :: "constraint \<Rightarrow> string set" where
+  "c_fv (Constraint ms ms' msg) = \<Union>(m_fv ` (set ms \<union> set ms' \<union> {msg}))"
+
+fun c_sapply :: "m_subst \<Rightarrow> constraint \<Rightarrow> constraint" where
+  "c_sapply \<sigma> (Constraint ms ms' msg) = Constraint (map (m_sapply \<sigma>) ms) (map (m_sapply \<sigma>) ms') (m_sapply \<sigma> msg)"
+
+fun c_derives :: "constraint \<Rightarrow> bool" where
+  "c_derives (Constraint ms ms' msg) = (set ms \<union> set ms') \<turnstile> msg"
+
+lemma "c_sapply_comp": "c_sapply \<tau> (c_sapply \<sigma> c) = c_sapply (\<tau> \<circ>m \<sigma>) c"
+  using m_sapply_comp
+  by (cases c) simp
+
+definition cs_fv :: "constraint_sys \<Rightarrow> string set" where
+  "cs_fv cs = \<Union>(c_fv ` cs)"
+
+definition cs_sapply :: "m_subst \<Rightarrow> constraint_sys \<Rightarrow> constraint_sys" where
+  "cs_sapply \<sigma> cs = c_sapply \<sigma> ` cs"
+
+fun cs_derives :: "constraint_sys \<Rightarrow> bool" where
+  "cs_derives cs = (\<forall>c \<in> cs. c_derives c)"
+
+(* 7. (b) *)
+
+type_synonym sol_set = "m_subst set"
+definition sol :: "constraint_sys \<Rightarrow> sol_set" where
+  "sol cs = {\<sigma> | \<sigma>. cs_derives (cs_sapply \<sigma> cs)}"
+
+lemma "sol_cs_union": "sol (cs \<union> cs') = (sol cs) \<inter> (sol cs')"
+  unfolding sol_def cs_sapply_def
+  by (rule set_eqI) auto
+
+lemma "sol_subst_comp": "\<tau> \<in> sol (cs_sapply \<sigma> cs) \<Longrightarrow> \<tau> \<circ>m \<sigma> \<in> sol cs"
+  unfolding sol_def cs_sapply_def
+  using c_sapply_comp by auto
 
 end
